cleanup

src/test.ec
@@ -1,39 +1,22 @@
 pragma Goals:printall.
 require import Int Logic IntDiv CoreMap SmtMap.
 
-type MemoryMap = (int, int) map.
-
-
+type uint256 = int.
+type MemoryMap = (uint256, uint256) map.
 
 op p = 21888242871839275222246405745257275088696311157297823662689037894645226208583.
 
-(*
-op "_.[_<-_]" ['a, 'b] (f : 'a -> 'b) (x : 'a) (y : 'b) =
-  fun x' => if x = x' then y else f x'.
-
-lemma fupdateE ['a 'b] (f : 'a -> 'b) (x x' : 'a) (y : 'b) :
-  f.[x <- y] x' = if x = x' then y else f x'.
-proof. by []. qed.
-
-lemma fupdate_eq ['a 'b] (f : 'a -> 'b) (x : 'a) (y : 'b) :
-  f.[x <- y] x = y.
-proof. by []. qed.
-
-lemma fupdate_neq ['a 'b] (f : 'a -> 'b) (x x' : 'a) (y : 'b) :
-  x <> x' => f.[x <- y] x' = f x'.
-proof. by move=> @/"_.[_<-_]" ->. qed.
-*)
 module Test = {
 
-  proc mload(m : MemoryMap, a : int) : int = {
+  proc mload(m : MemoryMap, a : uint256) : uint256 = {
     return m.[a];
   }
 
-  proc mstore(m : MemoryMap, a : int, v : int) : MemoryMap = {
+  proc mstore(m : MemoryMap, a : uint256, v : uint256) : MemoryMap = {
     return m.[a<-v];
   }
   
-  proc pointNegate(m : MemoryMap, point : int): MemoryMap = {
+  proc pointNegate(m : MemoryMap, point : uint256): MemoryMap = {
       var _1, _2, _3, pY, tmp166, tmp167, tmp168, _6, _7, tmp170;
       _1 <- 32;
       _2 <- point + _1;
@@ -54,28 +37,13 @@ module Test = {
           tmp170 <@ mstore(m, _2, _7);
       }
       return tmp170;
-  }
-
-  proc stupid(a : int, b : int) : int = {
-    return a + b;
-  }
+    }
   
 }.
-
-lemma stupid_lemma :
-    forall (a b : int), hoare[ Test.stupid : arg = (a,b) ==> res = a + b].
-    progress.
-    proc.
-    skip.
-    progress.
-    qed.
-
-print ( < ).
     
 lemma pointNegate_lemma :
-    forall (m : MemoryMap) (point_addr : int),
-    m.[point_addr] <> 0 \/ m.[point_addr + 32] <> 0 => m.[point_addr + 32] < p
-    => 0 < m.[point_addr + 32] =>
+    forall (m : MemoryMap) (point_addr : uint256),
+    (m.[point_addr] <> 0 \/ m.[point_addr + 32] <> 0) /\ m.[point_addr + 32] < p /\ 0 < m.[point_addr + 32] =>
         hoare [ Test.pointNegate : arg = (m, point_addr) ==>
           (m.[point_addr] = res.[point_addr] /\ res.[point_addr + 32] = (-m.[point_addr + 32]) %% p)]. 
             progress.
@@ -90,10 +58,7 @@ lemma pointNegate_lemma :
             smt.
             rewrite -/p.
             smt.
-qed.            
+            qed.            
             
-        
-        
-        
-        
-        
+
+            
